tools/c-parser/Simpl/SmallStep.thy
@@ -1,29 +1,8 @@
 (*
     Author:      Norbert Schirmer
     Maintainer:  Norbert Schirmer, norbert.schirmer at web de
-    License:     LGPL
-*)
-
-(*  Title:      SmallStep.thy
-    Author:     Norbert Schirmer, TU Muenchen
 
 Copyright (C) 2006-2008 Norbert Schirmer
-Some rights reserved, TU Muenchen
-
-This library is free software; you can redistribute it and/or modify
-it under the terms of the GNU Lesser General Public License as
-published by the Free Software Foundation; either version 2.1 of the
-License, or (at your option) any later version.
-
-This library is distributed in the hope that it will be useful, but
-WITHOUT ANY WARRANTY; without even the implied warranty of
-MERCHANTABILITY or FITNESS FOR A PARTICULAR PURPOSE. See the GNU
-Lesser General Public License for more details.
-
-You should have received a copy of the GNU Lesser General Public
-License along with this library; if not, write to the Free Software
-Foundation, Inc., 59 Temple Place, Suite 330, Boston, MA 02111-1307
-USA
 *)
 
 section \<open>Small-Step Semantics and Infinite Computations\<close>
