tools/c-parser/Simpl/StateSpace.thy
@@ -1,29 +1,10 @@
 (*
     Author:      Norbert Schirmer
     Maintainer:  Norbert Schirmer, norbert.schirmer at web de
-    License:     LGPL
-*)
-
-(*  Title:      StateSpace.thy
-    Author:     Norbert Schirmer, TU Muenchen
 
 Copyright (C) 2004-2008 Norbert Schirmer
-Some rights reserved, TU Muenchen
+Copyright (c) 2022 Apple Inc. All rights reserved.
 
-This library is free software; you can redistribute it and/or modify
-it under the terms of the GNU Lesser General Public License as
-published by the Free Software Foundation; either version 2.1 of the
-License, or (at your option) any later version.
-
-This library is distributed in the hope that it will be useful, but
-WITHOUT ANY WARRANTY; without even the implied warranty of
-MERCHANTABILITY or FITNESS FOR A PARTICULAR PURPOSE. See the GNU
-Lesser General Public License for more details.
-
-You should have received a copy of the GNU Lesser General Public
-License along with this library; if not, write to the Free Software
-Foundation, Inc., 59 Temple Place, Suite 330, Boston, MA 02111-1307
-USA
 *)
 
 section \<open>State Space Template\<close>
@@ -37,10 +18,21 @@ definition
 where
   "upd_globals upd s = s\<lparr>globals := upd (globals s)\<rparr>"
 
+named_theorems state_simp
+
+lemma upd_globals_conv [state_simp]: "upd_globals f = (\<lambda>s. s\<lparr>globals := f (globals s)\<rparr>)"
+  by (rule ext) (simp add: upd_globals_def)
+
+record ('g, 'l) state_locals = "'g state" +
+  locals :: 'l
+
+(*
 record ('g, 'n, 'val) stateSP = "'g state" +
   locals :: "'n \<Rightarrow> 'val"
+*)
 
-lemma upd_globals_conv: "upd_globals f = (\<lambda>s. s\<lparr>globals := f (globals s)\<rparr>)"
-  by (rule ext) (simp add: upd_globals_def)
+type_synonym ('g, 'n, 'val) stateSP = "('g, 'n \<Rightarrow> 'val) state_locals"
+type_synonym ('g, 'n, 'val, 'x) stateSP_scheme = "('g, 'n \<Rightarrow> 'val, 'x) state_locals_scheme"
+
 
 end
